theories/cast_calculus/consistency/equivalence/intermediate.v
@@ -2,64 +2,92 @@ From stdpp Require Import base list.
 From Autosubst Require Export Autosubst.
 Require Export Utf8_core.
 
-From fae_gtlc_mu.equivalence Require Import types.
+From fae_gtlc_mu.cast_calculus Require Import types.
 
 Inductive cons_struct_pre (A : list (type * type)) : type -> type -> Type :=
   (** ground and star *)
   (* downcasting from star to ground *)
-  | consStarTGround τG
+  | consp_StarTGround τG
       (G : Ground τG) :
       cons_struct_pre A TUnknown τG
   (* upcasting from ground to star *)
-  | consTGroundStar τG
+  | consp_TGroundStar τG
       (G : Ground τG) :
       cons_struct_pre A τG TUnknown
   (** factorization through ground types, first direction *)
-  | consTauGroundArrow (τ1 τ2 : type)
+  | consp_TauGroundProd (τ1 τ2 : type)
+      (pτnG : τ1 ≠ TUnknown ∨ τ2 ≠ TUnknown)
+      (pC1 : cons_struct_pre A τ1 TUnknown)
+      (pC2 : cons_struct_pre A τ2 TUnknown) :
+      cons_struct_pre A (TProd τ1 τ2) TUnknown 
+  | consp_TauGroundSum (τ1 τ2 : type)
+      (pτnG : τ1 ≠ TUnknown ∨ τ2 ≠ TUnknown)
+      (pC1 : cons_struct_pre A τ1 TUnknown)
+      (pC2 : cons_struct_pre A τ2 TUnknown) :
+      cons_struct_pre A (TSum τ1 τ2) TUnknown 
+  | consp_TauGroundArrow (τ1 τ2 : type)
       (pτnG : τ1 ≠ TUnknown ∨ τ2 ≠ TUnknown)
       (pC1 : cons_struct_pre A TUnknown τ1)
       (pC2 : cons_struct_pre A τ2 TUnknown) :
       cons_struct_pre A (TArrow τ1 τ2) TUnknown
-  | consTauGroundRecUseCall (τb : type) i
+  | consp_TauGroundRecUseCall (τb : type) i
       (pτnG : τb ≠ TUnknown)
       (pμτlμtrinA : A !! i = Some (TRec τb, TRec TUnknown)) :
       cons_struct_pre A (TRec τb) TUnknown
-  | consTauGroundRecExposeCall (τb : type)
+  | consp_TauGroundRecExposeCall (τb : type)
       (pτnG : τb ≠ TUnknown)
       (pμτlμτrnotA : (TRec τb, TRec TUnknown) ∉ A)
       (pUnfτlUnfτr : cons_struct_pre ((TRec τb, TRec TUnknown) :: A) τb.[TRec τb/] TUnknown) :
       cons_struct_pre A (TRec τb) TUnknown
   (** factorization through ground types, second direction *)
-  | consGroundArrowTau (τ1 τ2 : type)
+  | consp_GroundProdTau (τ1 τ2 : type)
+      (pτnG : τ1 ≠ TUnknown ∨ τ2 ≠ TUnknown)
+      (pC1 : cons_struct_pre A TUnknown τ1)
+      (pC2 : cons_struct_pre A TUnknown τ2) :
+      cons_struct_pre A TUnknown (TProd τ1 τ2)
+    | consp_GroundSumTau (τ1 τ2 : type)
+      (pτnG : τ1 ≠ TUnknown ∨ τ2 ≠ TUnknown)
+      (pC1 : cons_struct_pre A TUnknown τ1)
+      (pC2 : cons_struct_pre A TUnknown τ2) :
+      cons_struct_pre A TUnknown (TSum τ1 τ2)
+    | consp_GroundArrowTau (τ1 τ2 : type)
       (pτnG : τ1 ≠ TUnknown ∨ τ2 ≠ TUnknown)
       (pC1 : cons_struct_pre A τ1 TUnknown)
       (pC2 : cons_struct_pre A TUnknown τ2) :
       cons_struct_pre A TUnknown (TArrow τ1 τ2)
-  | consGroundRecTauUseCall (τb : type) i
+  | consp_GroundRecTauUseCall (τb : type) i
       (pτnG : τb ≠ TUnknown)
       (pμτlμtrinA : A !! i = Some (TRec TUnknown, TRec τb)) :
       cons_struct_pre A TUnknown (TRec τb)
-  | consGroundRecTauExposeCall (τb : type)
+  | consp_GroundRecTauExposeCall (τb : type)
       (pτnG : τb ≠ TUnknown)
       (pμτlμτrnotA : (TRec TUnknown , TRec τb) ∉ A)
       (pUnfτlUnfτr : cons_struct_pre ((TRec TUnknown, TRec τb) :: A) TUnknown τb.[TRec τb/]) :
       cons_struct_pre A TUnknown (TRec τb)
   (** identiy casts between Base and TUnknown *)
-  | consBaseBase :
+  | consp_BaseBase :
       cons_struct_pre A TUnit TUnit
-  | consStarStar :
+  | consp_StarStar :
       cons_struct_pre A TUnknown TUnknown
   (** between types of same structure *)
-  | consTArrowTArrow τ1 τ1' τ2 τ2'
+  | consp_TProdTProd τ1 τ1' τ2 τ2'
+      (pCons31 : cons_struct_pre A τ1 τ1')
+      (pCons24 : cons_struct_pre A τ2 τ2') :
+      cons_struct_pre A (TProd τ1 τ2) (TProd τ1' τ2')
+  | consp_TSumTSum τ1 τ1' τ2 τ2'
+      (pCons31 : cons_struct_pre A τ1 τ1')
+      (pCons24 : cons_struct_pre A τ2 τ2') :
+      cons_struct_pre A (TSum τ1 τ2) (TSum τ1' τ2')
+  | consp_TArrowTArrow τ1 τ1' τ2 τ2'
       (pCons31 : cons_struct_pre A τ1' τ1)
       (pCons24 : cons_struct_pre A τ2 τ2') :
       cons_struct_pre A (TArrow τ1 τ2) (TArrow τ1' τ2')
   (** exposing recursive calls *)
-  | consTRecTRecExposeCall τl τr
+  | consp_TRecTRecExposeCall τl τr
       (pμτlμτrnotA : (TRec τl, TRec τr) ∉ A)
       (pUnfτlUnfτr : cons_struct_pre ((TRec τl, TRec τr) :: A) τl.[TRec τl/] τr.[TRec τr/]) :
       cons_struct_pre A (TRec τl) (TRec τr)
   (** using recursive calls *)
-  | consTRecTRecUseCall τl τr i
+  | consp_TRecTRecUseCall τl τr i
       (pμτlμtrinA : A !! i = Some (TRec τl, TRec τr)) :
       cons_struct_pre A (TRec τl) (TRec τr).
