theories/cast_calculus/consistency/equivalence/second_half.v
@@ -1,0 +1,57 @@
+From stdpp Require Import base list.
+From Autosubst Require Export Autosubst.
+Require Export Utf8_core.
+
+From fae_gtlc_mu.cast_calculus Require Import types consistency.structural consistency.equivalence.intermediate.
+
+Lemma cons_struct_pre_cons_struct A τ τ' : cons_struct_pre A τ τ' → cons_struct A τ τ'.
+Proof.
+  intro p. induction p; try by constructor.
+  - eapply consTauStar.
+    intro abs. inversion abs. destruct pτnG; by apply H.
+    intro abs. inversion abs. auto.
+    + by apply consTProdTProd.
+    + apply consTGroundStar. constructor.
+  - eapply consTauStar.
+    intro abs. inversion abs. destruct pτnG; by apply H.
+    intro abs. inversion abs. auto.
+    + by apply consTSumTSum.
+    + apply consTGroundStar. constructor.
+  - eapply consTauStar.
+    intro abs. inversion abs. destruct pτnG; by apply H.
+    intro abs. inversion abs. auto.
+    + by apply consTArrowTArrow.
+    + apply consTGroundStar. constructor.
+  - eapply consTauStar.
+    intro abs. inversion abs. by apply pτnG. auto. auto.
+    + by eapply consTRecTRecUseCall.
+    + apply consTGroundStar. constructor.
+  - eapply consTauStar.
+    intro abs. inversion abs. by apply pτnG. auto. auto.
+    + by eapply consTRecTRecExposeCall.
+    + apply consTGroundStar. constructor.
+  - eapply consStarTau.
+    intro abs. inversion abs. destruct pτnG; by apply H.
+    intro abs. inversion abs. auto.
+    + apply consStarTGround. constructor.
+    + by apply consTProdTProd.
+  - eapply consStarTau.
+    intro abs. inversion abs. destruct pτnG; by apply H.
+    intro abs. inversion abs. auto.
+    + apply consStarTGround. constructor.
+    + by apply consTSumTSum.
+  - eapply consStarTau.
+    intro abs. inversion abs. destruct pτnG; by apply H.
+    intro abs. inversion abs. auto.
+    + apply consStarTGround. constructor.
+    + by apply consTArrowTArrow.
+  - eapply consStarTau.
+    intro abs. inversion abs. by apply pτnG. auto. auto.
+    + apply consStarTGround. constructor.
+    + by eapply consTRecTRecUseCall.
+  - eapply consStarTau.
+    intro abs. inversion abs. by apply pτnG. auto. auto.
+    + apply consStarTGround. constructor.
+    + by eapply consTRecTRecExposeCall.
+  - by eapply consTRecTRecUseCall.
+Qed.
