theories/refinements/static_gradual/compat_cast/star_ground.v
@@ -1,13 +1,12 @@
-From fae_gtlc_mu.refinements.static_gradual Require Export logical_relation resources_right compat_easy help_left compat_cast.defs compat_cast.extract_embed.
+From fae_gtlc_mu.refinements.static_gradual Require Export logical_relation resources_right compat_easy help_left compat_cast.defs.
 From fae_gtlc_mu.stlc_mu Require Export lang.
 From fae_gtlc_mu.cast_calculus Require Export lang.
 From iris.algebra Require Import list.
 From iris.proofmode Require Import tactics.
 From iris.program_logic Require Import lifting.
 From fae_gtlc_mu.cast_calculus Require Export types.
-From fae_gtlc_mu.cast_calculus Require Export consistency.structural.definition.
+From fae_gtlc_mu.cast_calculus Require Export consistency.structural.
 From fae_gtlc_mu.backtranslation Require Export cast_help.general cast_help.extract cast_help.embed.
-From fae_gtlc_mu.refinements.static_gradual Require Export tactics_left.
 From fae_gtlc_mu.cast_calculus Require Export types typing.
 
 Section star_ground.
@@ -22,116 +21,157 @@ Section star_ground.
   Local Hint Resolve to_of_val : core.
   Local Hint Resolve stlc_mu.lang.to_of_val : core.
 
-  Lemma refold_interp_unknown' vv' : fixpoint interp_unknown1' vv' ≡ interp TUnknown [] vv'.
-  Proof.
-    auto.
-  Qed.
+  (* Lemma refold_interp_unknown' vv' : fixpoint interp_unknown1' vv' ≡ interp TUnknown [] vv'. *)
+  (* Proof. *)
+  (*   auto. *)
+  (* Qed. *)
 
 
   Lemma back_cast_ar_star_ground (A : list (type * type)) (τG : type) (G : Ground τG) : back_cast_ar (consStarTGround A τG G).
   Proof.
     rewrite /back_cast_ar /𝓕c /𝓕. iIntros (ei' K' v v' fs) "(#Hfs & #Hvv' & #Hei' & Hv')". rewrite extract_no_subs.
-    destruct G.
-    - (** TUnit *) rewrite unfold_fixpoint_interp_unknown1'; try by constructor.
-      iDestruct "Hvv'" as "[Hvv'Unit|[Hpp'|[Hss'|[Hff'|Huu']]]]".
-      * iDestruct "Hvv'Unit" as "%"; inversion H; clear v v' H H1 H2.
-        (** easy case; delegate to extract_embed file with good tactics *)
-
-        iApply wp_pure_step_later; auto; iNext; asimpl.
-        iApply (wp_bind (stlc_mu.lang.fill_item $ stlc_mu.lang.CaseCtx _ _)).
-        iApply wp_pure_step_later; auto; iNext.
-        iApply wp_value.
-        iApply wp_pure_step_later; auto; iNext.
-        iApply wp_pure_step_later; auto; iNext. asimpl.
-        iApply wp_pure_step_later; auto; iNext.
-        iApply wp_pure_step_later; auto; iNext. asimpl.
-        iMod (step_pure _ ei' K' (Cast (Cast Unit TUnit ⋆) ⋆ TUnit) (# UnitV) with "[Hv']") as "HHHH"; intros; auto.
-        apply Same_Ground with (v := UnitV ); auto; constructor.
-        iApply wp_value.
-        iExists UnitV.
-        by repeat iFrame.
-
-
-      * iDestruct "Hpp'" as (v1 v1' v2 v2') "(% & #H1 & #H2)". simpl in H; inversion H; clear H H1 H2 v v'.
-        repeat rewrite (refold_interp_unknown').
-        (** diverging case *)
-
-          asimpl.
-          iApply wp_pure_step_later; auto; iNext; asimpl.
-          iApply (wp_bind (stlc_mu.lang.fill_item $ stlc_mu.lang.CaseCtx _ _)).
-          iApply wp_pure_step_later; auto; iNext.
-          iApply wp_value.
-          iApply wp_pure_step_later; auto; iNext; asimpl.
-          iApply wp_pure_step_later; auto; iNext; asimpl.
-          iApply wp_pure_step_later; auto; iNext. asimpl.
-          by iApply wp_Ω.
-
-
-
-      * iDestruct "Hss'" as "[H1 | H2]".
-        -- iDestruct "H1" as (v1 v1') "[% Hv1v1']"; rewrite (refold_interp_unknown'); inversion H; clear H H1 H2 v v'.
-           (** diverging case *) admit.
-          -- iDestruct "H2" as (v2 v2') "[% Hv2v2']"; rewrite (refold_interp_unknown'); inversion H; clear H H1 H2 v v'.
-           (** diverging case *) admit.
-      * iDestruct "Hff'" as (f f') "[% Hff']". inversion H. clear H H1 H2 v v'.
-        (** diverging case *) admit.
-      * iDestruct "Huu'" as (u u') "[% H]"; rewrite (refold_interp_unknown'); inversion H; clear H H1 H2 v v'.
-        (** diverging case *) admit.
-    - (** TProd *)
-      admit.
-    - (** TSum *) admit.
-    - (** TArrow *) rewrite unfold_fixpoint_interp_unknown1'.
-      iDestruct "Hvv'" as "[Hvv'Unit|[Hpp'|[Hss'|[Hff'|Huu']]] ]".
-      * iDestruct "Hvv'Unit" as "%"; inversion H; clear v v' H H1 H2.
-        (** diverging case *) admit.
-      * iDestruct "Hpp'" as (v1 v1' v2 v2') "(% & #H1 & #H2)". simpl in H; inversion H; clear H H1 H2 v v'.
-        repeat rewrite (refold_interp_unknown').
-        (** diverging case *) admit.
-      * iDestruct "Hss'" as "[H1 | H2]".
-        -- iDestruct "H1" as (v1 v1') "[% Hv1v1']"; rewrite (refold_interp_unknown'); inversion H; clear H H1 H2 v v'.
-            (** diverging case *) admit.
-        -- iDestruct "H2" as (v2 v2') "[% Hv2v2']"; rewrite (refold_interp_unknown'); inversion H; clear H H1 H2 v v'.
-            (** diverging case *) admit.
-      * iDestruct "Hff'" as (f f') "[% Hff']". inversion H. clear H H1 H2 v v'.
-        (** easy case *) admit.
-      * iDestruct "Huu'" as (u u') "[% H]"; rewrite (refold_interp_unknown'); inversion H; clear H H1 H2 v v'.
-        (** diverging case *) admit.
-      * constructor.
-    - (** TRec *) rewrite unfold_fixpoint_interp_unknown1'.
-      iDestruct "Hvv'" as "[Hvv'Unit|[Hpp'|[Hss'|[Hff'|Huu']]] ]".
-      * iDestruct "Hvv'Unit" as "%"; inversion H; clear v v' H H1 H2.
-        (** diverging case *) admit.
-      * iDestruct "Hpp'" as (v1 v1' v2 v2') "(% & #H1 & #H2)". simpl in H; inversion H; clear H H1 H2 v v'.
-        repeat rewrite (refold_interp_unknown').
-        (** diverging case *) admit.
-      * iDestruct "Hss'" as "[H1 | H2]".
-        -- iDestruct "H1" as (v1 v1') "[% Hv1v1']"; rewrite (refold_interp_unknown'); inversion H; clear H H1 H2 v v'.
-           (** diverging case *) admit.
-        -- iDestruct "H2" as (v2 v2') "[% Hv2v2']"; rewrite (refold_interp_unknown'); inversion H; clear H H1 H2 v v'.
-           (** diverging case *) admit.
-      * iDestruct "Hff'" as (f f') "[% Hff']". inversion H. clear H H1 H2 v v'.
-        (** diverging case *) admit.
-      * iDestruct "Huu'" as (u u') "[% #H]"; rewrite (refold_interp_unknown'); inversion H; clear H H1 H2 v v'.
-        (** easy case*)
-        iMod (step_pure _ ei' K'
-                          (Cast (# castupV_TRec (FoldV u')) ⋆ (TRec ⋆))
-                          (# (FoldV u'))
-                  with "[Hv']") as "HHHH"; auto.
-          intro; eapply Same_Ground; simplify_option_eq; auto; constructor.
-          iApply wp_pure_step_later; auto; iNext; asimpl.
-          iApply (wp_bind (stlc_mu.lang.fill_item $ stlc_mu.lang.CaseCtx _ _)).
-          iApply wp_pure_step_later; auto.
-          iApply wp_value. simpl.
-          iApply wp_pure_step_later; auto. asimpl.
-          iApply wp_value.
-          repeat iNext.
-          iExists (FoldV u'). iSplitL. done.
-          rewrite fixpoint_interp_rec1_eq.
-          iModIntro.
-          iExists (u, u').
-          iSplitL; done.
-      * constructor.
+    destruct G; rewrite interp_rw_TUnknown.
+    - (iDestruct "Hvv'" as (w w') "#[[% Hww]|[[% Hww]|[[% Hww]|[[% Hww]|[% Hww]]]]]"; inversion H; clear H H1 H2 v v').
+      + admit.
+      + admit.
+      + admit.
+      + admit.
+      + admit.
+    - (iDestruct "Hvv'" as (w w') "#[[% Hww]|[[% Hww]|[[% Hww]|[[% Hww]|[% Hww]]]]]"; inversion H; clear H H1 H2 v v').
+      + admit.
+      + admit.
+      + admit.
+      + admit.
+      + admit.
+    - (iDestruct "Hvv'" as (w w') "#[[% Hww]|[[% Hww]|[[% Hww]|[[% Hww]|[% Hww]]]]]"; inversion H; clear H H1 H2 v v').
+      + admit.
+      + admit.
+      + admit.
+      + admit.
+      + admit.
+    - (iDestruct "Hvv'" as (w w') "#[[% Hww]|[[% Hww]|[[% Hww]|[[% Hww]|[% Hww]]]]]"; inversion H; clear H H1 H2 v v').
+      + admit.
+      + admit.
+      + admit.
+      + admit.
+      + admit.
+    - (iDestruct "Hvv'" as (w w') "#[[% Hww]|[[% Hww]|[[% Hww]|[[% Hww]|[% Hww]]]]]"; inversion H; clear H H1 H2 v v').
+      + admit.
+      + admit.
+      + admit.
+      + admit.
+      + admit.
+      + admit.
   Admitted.
+
+
+  (* Lemma back_cast_ar_star_ground (A : list (type * type)) (τG : type) (G : Ground τG) : back_cast_ar (consStarTGround A τG G). *)
+  (* Proof. *)
+  (*   rewrite /back_cast_ar /𝓕c /𝓕. iIntros (ei' K' v v' fs) "(#Hfs & #Hvv' & #Hei' & Hv')". rewrite extract_no_subs. *)
+  (*   destruct G. *)
+  (*   - (** TUnit *) rewrite unfold_fixpoint_interp_unknown1'; try by constructor. *)
+  (*     iDestruct "Hvv'" as "[Hvv'Unit|[Hpp'|[Hss'|[Hff'|Huu']]]]". *)
+  (*     * iDestruct "Hvv'Unit" as "%"; inversion H; clear v v' H H1 H2. *)
+  (*       (** easy case; delegate to extract_embed file with good tactics *) *)
+  (*       admit. *)
+
+  (*       (* iApply wp_pure_step_later; auto; iNext; asimpl. *) *)
+  (*       (* iApply (wp_bind (stlc_mu.lang.fill_item $ stlc_mu.lang.CaseCtx _ _)). *) *)
+  (*       (* iApply wp_pure_step_later; auto; iNext. *) *)
+  (*       (* iApply wp_value. *) *)
+  (*       (* iApply wp_pure_step_later; auto; iNext. *) *)
+  (*       (* iApply wp_pure_step_later; auto; iNext. asimpl. *) *)
+  (*       (* iApply wp_pure_step_later; auto; iNext. *) *)
+  (*       (* iApply wp_pure_step_later; auto; iNext. asimpl. *) *)
+  (*       (* iMod (step_pure _ ei' K' (Cast (Cast Unit TUnit ⋆) ⋆ TUnit) (# UnitV) with "[Hv']") as "HHHH"; intros; auto. *) *)
+  (*       (* apply Same_Ground with (v := UnitV ); auto; constructor. *) *)
+  (*       (* iApply wp_value. *) *)
+  (*       (* iExists UnitV. *) *)
+  (*       (* by repeat iFrame. *) *)
+
+
+  (*     * iDestruct "Hpp'" as (v1 v1' v2 v2') "(% & #H1 & #H2)". simpl in H; inversion H; clear H H1 H2 v v'. *)
+  (*       repeat rewrite (refold_interp_unknown'). *)
+  (*       (** diverging case *) *)
+  (*       admit. *)
+
+  (*         (* asimpl. *) *)
+  (*         (* iApply wp_pure_step_later; auto; iNext; asimpl. *) *)
+  (*         (* iApply (wp_bind (stlc_mu.lang.fill_item $ stlc_mu.lang.CaseCtx _ _)). *) *)
+  (*         (* iApply wp_pure_step_later; auto; iNext. *) *)
+  (*         (* iApply wp_value. *) *)
+  (*         (* iApply wp_pure_step_later; auto; iNext; asimpl. *) *)
+  (*         (* iApply wp_pure_step_later; auto; iNext; asimpl. *) *)
+  (*         (* iApply wp_pure_step_later; auto; iNext. asimpl. *) *)
+  (*         (* by iApply wp_Ω. *) *)
+
+
+
+  (*     * iDestruct "Hss'" as "[H1 | H2]". *)
+  (*       -- iDestruct "H1" as (v1 v1') "[% Hv1v1']"; rewrite (refold_interp_unknown'); inversion H; clear H H1 H2 v v'. *)
+  (*          (** diverging case *) admit. *)
+  (*         -- iDestruct "H2" as (v2 v2') "[% Hv2v2']"; rewrite (refold_interp_unknown'); inversion H; clear H H1 H2 v v'. *)
+  (*          (** diverging case *) admit. *)
+  (*     * iDestruct "Hff'" as (f f') "[% Hff']". inversion H. clear H H1 H2 v v'. *)
+  (*       (** diverging case *) admit. *)
+  (*     * iDestruct "Huu'" as (u u') "[% H]"; rewrite (refold_interp_unknown'); inversion H; clear H H1 H2 v v'. *)
+  (*       (** diverging case *) admit. *)
+  (*   - (** TProd *) *)
+  (*     admit. *)
+  (*   - (** TSum *) admit. *)
+  (*   - (** TArrow *) rewrite unfold_fixpoint_interp_unknown1'. *)
+  (*     iDestruct "Hvv'" as "[Hvv'Unit|[Hpp'|[Hss'|[Hff'|Huu']]] ]". *)
+  (*     * iDestruct "Hvv'Unit" as "%"; inversion H; clear v v' H H1 H2. *)
+  (*       (** diverging case *) admit. *)
+  (*     * iDestruct "Hpp'" as (v1 v1' v2 v2') "(% & #H1 & #H2)". simpl in H; inversion H; clear H H1 H2 v v'. *)
+  (*       repeat rewrite (refold_interp_unknown'). *)
+  (*       (** diverging case *) admit. *)
+  (*     * iDestruct "Hss'" as "[H1 | H2]". *)
+  (*       -- iDestruct "H1" as (v1 v1') "[% Hv1v1']"; rewrite (refold_interp_unknown'); inversion H; clear H H1 H2 v v'. *)
+  (*           (** diverging case *) admit. *)
+  (*       -- iDestruct "H2" as (v2 v2') "[% Hv2v2']"; rewrite (refold_interp_unknown'); inversion H; clear H H1 H2 v v'. *)
+  (*           (** diverging case *) admit. *)
+  (*     * iDestruct "Hff'" as (f f') "[% Hff']". inversion H. clear H H1 H2 v v'. *)
+  (*       (** easy case *) admit. *)
+  (*     * iDestruct "Huu'" as (u u') "[% H]"; rewrite (refold_interp_unknown'); inversion H; clear H H1 H2 v v'. *)
+  (*       (** diverging case *) admit. *)
+  (*     * constructor. *)
+  (*   - (** TRec *) rewrite unfold_fixpoint_interp_unknown1'. *)
+  (*     iDestruct "Hvv'" as "[Hvv'Unit|[Hpp'|[Hss'|[Hff'|Huu']]] ]". *)
+  (*     * iDestruct "Hvv'Unit" as "%"; inversion H; clear v v' H H1 H2. *)
+  (*       (** diverging case *) admit. *)
+  (*     * iDestruct "Hpp'" as (v1 v1' v2 v2') "(% & #H1 & #H2)". simpl in H; inversion H; clear H H1 H2 v v'. *)
+  (*       repeat rewrite (refold_interp_unknown'). *)
+  (*       (** diverging case *) admit. *)
+  (*     * iDestruct "Hss'" as "[H1 | H2]". *)
+  (*       -- iDestruct "H1" as (v1 v1') "[% Hv1v1']"; rewrite (refold_interp_unknown'); inversion H; clear H H1 H2 v v'. *)
+  (*          (** diverging case *) admit. *)
+  (*       -- iDestruct "H2" as (v2 v2') "[% Hv2v2']"; rewrite (refold_interp_unknown'); inversion H; clear H H1 H2 v v'. *)
+  (*          (** diverging case *) admit. *)
+  (*     * iDestruct "Hff'" as (f f') "[% Hff']". inversion H. clear H H1 H2 v v'. *)
+  (*       (** diverging case *) admit. *)
+  (*     * iDestruct "Huu'" as (u u') "[% #H]"; rewrite (refold_interp_unknown'); inversion H; clear H H1 H2 v v'. *)
+  (*       (** easy case*) *)
+  (*       rewrite /embedV_TUnknown /castupV_TRec. *)
+  (*       iMod (step_pure _ ei' K' *)
+  (*                         (Cast (# castupV_TRec (FoldV u')) ⋆ (TRec ⋆)) *)
+  (*                         (# (FoldV u')) *)
+  (*                 with "[Hv']") as "HHHH"; auto. *)
+  (*       eapply Same_Ground. apply to_of_val. constructor. *)
+  (*       iApply wp_pure_step_later; auto; iNext; asimpl. *)
+  (*       iApply (wp_bind (stlc_mu.lang.fill_item $ stlc_mu.lang.CaseCtx _ _)). *)
+  (*       iApply wp_pure_step_later; auto. *)
+  (*       iApply wp_value. simpl. *)
+  (*       iApply wp_pure_step_later; auto. asimpl. *)
+  (*       iApply wp_value. *)
+  (*       repeat iNext. *)
+  (*       iExists (FoldV u'). iSplitL. done. *)
+  (*       rewrite fixpoint_interp_rec1_eq. *)
+  (*       iModIntro. *)
+  (*       iExists (u, u'). *)
+  (*       iSplitL; done. *)
+  (*     * constructor. *)
+  (* Admitted. *)
 
 
 End star_ground.
